Update [DListLow.fst] to use the changes made in [DListRef.fst]

DListLow.fst
@@ -16,15 +16,13 @@ module HS = FStar.HyperStack
 module B = FStar.Buffer
 module ST = FStar.HyperStack.ST
 
-#set-options "--use_two_phase_tc true"
-
 unopteq
 (** Node of a doubly linked list *)
 type dlist (t:Type0) = {
   (* forward link *)
-  flink: (gpointer_or_null (dlist t));
+  flink: gpointer_or_null (dlist t);
   (* backward link *)
-  blink: (gpointer_or_null (dlist t));
+  blink: gpointer_or_null (dlist t);
   (* payload *)
   p: t;
 }
@@ -32,8 +30,8 @@ type dlist (t:Type0) = {
 unopteq
 (** Doubly linked list head *)
 type dlisthead (t:Type0) ={
-  lhead: (gpointer_or_null (dlist t));
-  ltail: (gpointer_or_null (dlist t));
+  lhead: gpointer_or_null (dlist t);
+  ltail: gpointer_or_null (dlist t);
   nodes: erased (seq (gpointer (dlist t)));
 }
 
@@ -51,36 +49,40 @@ val getSome: (a:gpointer_or_null 'a{is_not_null a}) -> (b:gpointer 'a{g_ptr_eq a
 let getSome a = a
 
 unfold let (@) (a:gpointer 't) (h0:HS.mem{h0 `B.live` a}) = B.get h0 a 0
-unfold let (^@) (a:(gpointer_or_null 't){is_not_null a}) (h0:HS.mem{h0 `B.live` (getSome a)}) = (getSome a) @ h0
+unfold let (^@) (a:gpointer_or_null 't{is_not_null a}) (h0:HS.mem{h0 `B.live` (getSome a)}) = (getSome a) @ h0
 
 unfold let (.[]) (s:seq 'a) (n:nat{n < length s}) = index s n
 
 // logic : Cannot use due to https://github.com/FStarLang/FStar/issues/638
-let not_aliased (#t:Type) (a:(gpointer_or_null t)) (b:(gpointer_or_null t)) : GTot Type0 =
+let not_aliased (#t:Type) (a:gpointer_or_null t) (b:gpointer_or_null t) : GTot Type0 =
   is_null a \/ is_null b \/
-  disjoint (getSome a) (getSome b)
+  (let (a:_{is_not_null a}) = a in // workaround for not using two phase type checker
+   let (b:_{is_not_null b}) = b in
+   disjoint (getSome a) (getSome b))
 
 // logic : Cannot use due to https://github.com/FStarLang/FStar/issues/638
-let not_aliased0 (#t:Type) (a:gpointer t) (b:(gpointer_or_null t)) : GTot Type0 =
+let not_aliased0 (#t:Type) (a:gpointer t) (b:gpointer_or_null t) : GTot Type0 =
   is_null b \/
-  disjoint a (getSome b)
+  (let (b:_{is_not_null b}) = b in // workaround for not using two phase type checker
+   disjoint a (getSome b))
 
 logic
 let not_aliased00 (#t:Type) (a:gpointer t) (b:gpointer t) : GTot Type0 =
   disjoint a b
 
-// logic
+logic
 let dlist_is_valid' (#t:Type) (h0:HS.mem) (n:dlist t) : GTot Type0 =
   not_aliased n.flink n.blink
 
 // logic
 let dlist_is_valid (#t:Type) (h0:HS.mem) (n:gpointer (dlist t)) : GTot Type0 =
   h0 `B.live` n /\
-  dlist_is_valid' #t h0 (n@h0)
+  dlist_is_valid' h0 (n@h0)
 
-let (==$) (#t:Type) (a:(gpointer_or_null t)) (b:gpointer t) =
+let (==$) (#t:Type) (a:gpointer_or_null t) (b:gpointer t) =
   is_not_null a /\
-  g_ptr_eq (getSome a) b
+  (let (a:_{is_not_null a}) = a in // workaround for not using two phase type checker
+   g_ptr_eq (getSome a) b)
 
 logic
 let ( |> ) (#t:Type) (a:dlist t) (b:gpointer (dlist t)) : GTot Type0 =
@@ -90,6 +92,7 @@ logic
 let ( <| ) (#t:Type) (a:gpointer (dlist t)) (b: dlist t) : GTot Type0 =
   b.blink ==$ a
 
+irreducible
 let ( =|> ) (#t:Type) (a:gpointer (dlist t)) (b:gpointer (dlist t)) : ST unit
     (requires (fun h0 ->
          h0 `B.live` a /\ h0 `B.live` b /\
@@ -104,6 +107,7 @@ let ( =|> ) (#t:Type) (a:gpointer (dlist t)) (b:gpointer (dlist t)) : ST unit
          (a@h2) |> b)) =
   a := { !a with flink = b }
 
+irreducible
 let ( <|= ) (#t:Type) (a:gpointer (dlist t)) (b:gpointer (dlist t)) : ST unit
     (requires (fun h0 ->
          h0 `B.live` a /\ h0 `B.live` b /\
@@ -118,6 +122,7 @@ let ( <|= ) (#t:Type) (a:gpointer (dlist t)) (b:gpointer (dlist t)) : ST unit
          a <| (b@h2))) =
   b := { !b with blink = a }
 
+irreducible
 let ( !=|> ) (#t:Type) (a:gpointer (dlist t)) : ST unit
     (requires (fun h0 -> h0 `B.live` a))
     (ensures (fun h1 _ h2 ->
@@ -128,6 +133,7 @@ let ( !=|> ) (#t:Type) (a:gpointer (dlist t)) : ST unit
          (a@h2).flink == null)) =
   a := { !a with flink = null }
 
+irreducible
 let ( !<|= ) (#t:Type) (a:gpointer (dlist t)) : ST unit
     (requires (fun h0 -> h0 `B.live` a))
     (ensures (fun h1 _ h2 ->
@@ -155,18 +161,18 @@ let flink_valid (#t:Type) (h0:HS.mem) (h:dlisthead t) : GTot Type0 =
   let nodes = reveal h.nodes in
   let len = length nodes in
   all_nodes_contained h0 h /\
-  (forall i j. {:pattern ((nodes.[i]@h0).flink); (nodes.[j])}
-     ((0 <= i /\ i < len - 1 /\ j = i+1) ==>
-      (nodes.[i]@h0 |> nodes.[j])))
+  (forall i. {:pattern ((nodes.[i]@h0).flink)}
+     ((0 <= i /\ i < len - 1) ==>
+      nodes.[i]@h0 |> nodes.[i+1]))
 
 logic
 let blink_valid (#t:Type) (h0:HS.mem) (h:dlisthead t) : GTot Type0 =
   let nodes = reveal h.nodes in
   let len = length nodes in
   all_nodes_contained h0 h /\
-  (forall i j. {:pattern ((nodes.[i]@h0).blink); (nodes.[j])}
-     ((1 <= i /\ i < len /\ j=i-1) ==>
-      (nodes.[j] <| nodes.[i]@h0)))
+  (forall i. {:pattern ((nodes.[i]@h0).blink)}
+     ((1 <= i /\ i < len) ==>
+      nodes.[i-1] <| nodes.[i]@h0))
 
 logic
 let dlisthead_ghostly_connections (#t:Type) (h0:HS.mem) (h:dlisthead t) : GTot Type0 =
@@ -186,7 +192,7 @@ let elements_dont_alias1 (#t:Type) (h0:HS.mem) (h:dlisthead t) : GTot Type0 =
   all_nodes_contained h0 h /\
   (forall i j. {:pattern (not_aliased (nodes.[i]@h0).flink (nodes.[j]@h0).flink)}
      0 <= i /\ i < j /\ j < length nodes ==>
-   (not_aliased (nodes.[i]@h0).flink (nodes.[j]@h0).flink))
+   not_aliased (nodes.[i]@h0).flink (nodes.[j]@h0).flink)
 
 logic
 let elements_dont_alias2 (#t:Type) (h0:HS.mem) (h:dlisthead t) : GTot Type0 =
@@ -194,7 +200,7 @@ let elements_dont_alias2 (#t:Type) (h0:HS.mem) (h:dlisthead t) : GTot Type0 =
   all_nodes_contained h0 h /\
   (forall i j. {:pattern (not_aliased (nodes.[i]@h0).blink (nodes.[j]@h0).blink)}
      0 <= i /\ i < j /\ j < length nodes ==>
-   (not_aliased (nodes.[i]@h0).blink (nodes.[j]@h0).blink))
+   not_aliased (nodes.[i]@h0).blink (nodes.[j]@h0).blink)
 
 // logic : Cannot use due to https://github.com/FStarLang/FStar/issues/638
 let elements_dont_alias (#t:Type) (h0:HS.mem) (h:dlisthead t) : GTot Type0 =
@@ -211,11 +217,13 @@ let elements_are_valid (#t:Type) (h0:HS.mem) (h:dlisthead t) : GTot Type0 =
 logic
 let all_elements_distinct (#t:Type) (h0:HS.mem) (h:dlisthead t) : GTot Type0 =
     let nodes = reveal h.nodes in
-    (forall i j. {:pattern (nodes.[i]); (nodes.[j])}
+    (forall i j. {:pattern (disjoint nodes.[i] nodes.[j])}
        (0 <= i /\ i < j /\ j < Seq.length nodes) ==>
-       (disjoint nodes.[i] nodes.[j]))
+       (let (i:nat{i < Seq.length nodes}) = i in // workaround for not using two phase type checker
+        let (j:nat{j < Seq.length nodes}) = j in
+        disjoint nodes.[i] nodes.[j]))
 
-logic
+unfold logic
 let dlisthead_is_valid (#t:Type) (h0:HS.mem) (h:dlisthead t) : GTot Type0 =
   let nodes = reveal h.nodes in
   let len = length nodes in
@@ -225,8 +233,49 @@ let dlisthead_is_valid (#t:Type) (h0:HS.mem) (h:dlisthead t) : GTot Type0 =
               flink_valid h0 h /\
               blink_valid h0 h) /\
   elements_are_valid h0 h /\
-  elements_dont_alias h0 h /\
-  all_elements_distinct h0 h
+  elements_dont_alias h0 h
+
+let rec two_elements_distinct (#t:Type) (h0:HS.mem) (h:dlisthead t) (i j:int) : Lemma
+  (requires (0 <= i /\ i < j /\ j < Seq.length (reveal h.nodes)) /\
+	    ~(length (reveal h.nodes) == 0) /\
+            dlisthead_ghostly_connections h0 h /\
+            flink_valid h0 h /\
+            blink_valid h0 h /\
+	    elements_are_valid h0 h /\
+	    elements_dont_alias h0 h)
+  (ensures
+     (let nodes = reveal h.nodes in
+      let (i:nat{i < Seq.length nodes}) = i in // workaround for not using two phase type checker
+      let (j:nat{j < Seq.length nodes}) = j in
+      disjoint nodes.[i] nodes.[j])) =
+  let nodes = reveal h.nodes in
+  if 0 <= i && i < j && j < Seq.length nodes then (
+    let b = FStar.StrongExcludedMiddle.strong_excluded_middle (disjoint nodes.[i] nodes.[j]) in
+    if not b then (
+      if i = 0 then (
+	assert( is_null (nodes.[i]@h0).blink);
+        assert( is_not_null (nodes.[j]@h0).blink)
+      ) else (
+	two_elements_distinct h0 h (i - 1) (j - 1)
+      )
+    ) else ()
+  ) else ()
+
+let lemma_all_elements_distinct (#t:Type) (h0:HS.mem) (h:dlisthead t) : Lemma
+    (requires dlisthead_is_valid h0 h)
+    (ensures all_elements_distinct h0 h) =
+  let nodes = reveal h.nodes in
+  let two_elements_distinct_helper (i j:int) : Lemma
+    ((0 <= i /\ i < j /\ j < Seq.length nodes) ==>
+       (let (i:nat{i < Seq.length nodes}) = i in // workaround for not using two phase type checker
+        let (j:nat{j < Seq.length nodes}) = j in
+        disjoint nodes.[i] nodes.[j]))
+    =
+    if 0 <= i && i < j && j < Seq.length nodes then (
+      two_elements_distinct h0 h i j
+    ) else ()
+  in
+  FStar.Classical.forall_intro_2 two_elements_distinct_helper
 
 let test1 () : Tot unit = assert (forall h0 t. dlisthead_is_valid h0 (empty_list #t))
 
@@ -240,7 +289,7 @@ let singletonlist #t e =
 
 // logic
 let contains_by_addr (#t:Type) (s:seq (gpointer t)) (x:gpointer t) : GTot Type0 =
-  (exists i. s.[i] == x)
+  (exists i. g_ptr_eq s.[i] x)
 
 logic
 let member_of (#t:eqtype) (h0:HS.mem) (h:dlisthead t) (e:gpointer (dlist t)) : GTot Type0 =
@@ -267,19 +316,24 @@ let has_nothing_in (#t:eqtype) (h0:HS.mem)
 
 type nonempty_dlisthead t = (h:dlisthead t{is_not_null h.lhead /\ is_not_null h.ltail})
 
-let ghost_is_singleton (#t:Type) (h:nonempty_dlisthead t) : GTot bool =
-  g_ptr_eq (getSome h.lhead) (getSome h.ltail)
+val dlisthead_make_valid_singleton: #t:eqtype -> h:nonempty_dlisthead t ->
+  ST (dlisthead t)
+    (requires (fun h0 ->
+         h0 `B.live` (getSome h.lhead) /\
+         is_null (h.lhead^@h0).flink /\ is_null (h.lhead^@h0).blink))
+    (ensures (fun h1 y h2 -> modifies_none h1 h2 /\ dlisthead_is_valid h2 y))
+let dlisthead_make_valid_singleton #t h =
+  let e = h.lhead in
+  { h with ltail = h.lhead ; nodes = ~. e }
 
-let is_singleton (#t:Type) (h:nonempty_dlisthead t) : ST bool
-    (requires (fun h0 -> h0 `B.live` h.lhead /\ h0 `B.live` h.ltail))
-    (ensures (fun h0 b h1 -> h0 == h1 /\ (b <==> ghost_is_singleton h))) =
-  ptr_eq (getSome h.lhead) (getSome h.ltail)
+let is_singleton (#t:Type) (h:nonempty_dlisthead t) : GTot Type0 =
+  g_ptr_eq (getSome h.lhead) (getSome h.ltail)
 
 val nonempty_singleton_properties :
   #t:Type ->
   h:nonempty_dlisthead t ->
   ST unit
-    (requires (fun h0 -> dlisthead_is_valid h0 h /\ ghost_is_singleton h))
+    (requires (fun h0 -> dlisthead_is_valid h0 h /\ is_singleton h))
     (ensures (fun h0 _ h1 -> h0 == h1 /\ Seq.length (reveal h.nodes) == 1))
 let nonempty_singleton_properties #t h = ()
 
@@ -287,7 +341,7 @@ val nonempty_nonsingleton_properties :
   #t:Type ->
   h:nonempty_dlisthead t ->
   ST unit
-    (requires (fun h0 -> dlisthead_is_valid h0 h /\ ~(ghost_is_singleton h)))
+    (requires (fun h0 -> dlisthead_is_valid h0 h /\ ~(g_ptr_eq (getSome h.lhead) (getSome h.ltail))))
     (ensures (fun h0 _ h1 -> h0 == h1 /\ Seq.length (reveal h.nodes) > 1))
 let nonempty_nonsingleton_properties #t h = ()
 
@@ -302,15 +356,12 @@ let ghost_append_properties #t a b = ()
 val dlisthead_update_head: #t:eqtype -> h:nonempty_dlisthead t -> e:gpointer (dlist t) ->
   ST (dlisthead t)
     (requires (fun h0 -> dlisthead_is_valid h0 h /\ dlist_is_valid h0 e /\ has_nothing_in h0 h e))
-    (ensures (fun h1 y h2 -> modifies_2 e (getSome h.lhead) h1 h2
-                             /\ dlisthead_is_valid h2 y))
+    (ensures (fun h1 y h2 -> modifies_2 e (getSome h.lhead) h1 h2 /\ dlisthead_is_valid h2 y))
 let dlisthead_update_head (#t:eqtype) (h:nonempty_dlisthead t) (e:gpointer (dlist t)) =
-  let h1 = ST.get () in
   let n = h.lhead in
   !<|= e;
   e =|> n;
   e <|= n;
-  admit ();
   { lhead = e ; ltail = h.ltail ; nodes = e ^+ h.nodes }
 
 #reset-options
@@ -336,13 +387,11 @@ val dlisthead_update_tail: #t:eqtype -> h:nonempty_dlisthead t -> e:gpointer (dl
     (requires (fun h0 -> dlisthead_is_valid h0 h /\ dlist_is_valid h0 e /\ has_nothing_in h0 h e))
     (ensures (fun h1 y h2 -> modifies_2 e (getSome h.ltail) h1 h2 /\ dlisthead_is_valid h2 y))
 let dlisthead_update_tail #t h e =
-  let h1 = ST.get () in
   let previously_singleton = is_singleton h in
   let n = h.ltail in
   !=|> e;
   n =|> e;
   n <|= e;
-  admit ();
   { lhead = h.lhead ; ltail = e ; nodes = h.nodes +^ e }
 
 #reset-options
@@ -364,19 +413,18 @@ let insertTailList #t h e =
 unfold let ghost_tail (#t:Type) (s:erased (seq t){Seq.length (reveal s) > 0}) : Tot (erased (seq t)) =
   hide (Seq.tail (reveal s))
 
-#set-options "--z3rlimit 50 --max_fuel 4 --max_ifuel 1"
+#set-options "--z3rlimit 100"
 
 val dlisthead_remove_head: #t:eqtype -> h:nonempty_dlisthead t ->
   ST (dlisthead t)
     (requires (fun h0 -> dlisthead_is_valid h0 h))
     (ensures (fun h1 y h2 ->
-         (ghost_is_singleton h ==>
           modifies_1 (getSome h.lhead) h1 h2) /\
-         (~(ghost_is_singleton h) ==>
           modifies_2 (getSome h.lhead) (reveal h.nodes).[1] h1 h2) /\
+         (is_singleton h ==>
+         (~(is_singleton h) ==>
          dlisthead_is_valid h2 y))
 let dlisthead_remove_head #t h =
-  let h1 = ST.get () in
   let n = h.lhead in
   if is_singleton h
   then (
@@ -387,17 +435,7 @@ let dlisthead_remove_head #t h =
     // unlink them
     !=|> n;
     !<|= next;
-    let htail = h.ltail in
-    let y = { lhead = next ; ltail = h.ltail ; nodes = ghost_tail h.nodes } in
-    let h2 = ST.get () in
-    assert (
-      let ynodes = reveal y.nodes in
-      let hnodes = reveal h.nodes in
-      (forall (i:nat{1 <= i /\ i < Seq.length ynodes /\ i+1 < Seq.length hnodes}).
-                {:pattern (ynodes.[i]@h2)}
-         ynodes.[i]@h2 == hnodes.[i+1]@h1)); // OBSERVE
-    admit ();
-      y
+    { lhead = next ; ltail = h.ltail ; nodes = ghost_tail h.nodes }
   )
 
 #reset-options
@@ -413,14 +451,13 @@ val dlisthead_remove_tail: #t:eqtype -> h:nonempty_dlisthead t ->
   ST (dlisthead t)
     (requires (fun h0 -> dlisthead_is_valid h0 h))
     (ensures (fun h1 y h2 ->
-         (ghost_is_singleton h ==>
+         (is_singleton h ==>
           modifies_1 (getSome h.ltail) h1 h2) /\
-         (~(ghost_is_singleton h) ==>
+         (~(is_singleton h) ==>
           (let nodes = reveal h.nodes in
           modifies_2 (getSome h.ltail) nodes.[length nodes - 2] h1 h2)) /\
          dlisthead_is_valid h2 y))
 let dlisthead_remove_tail #t h =
-  let h1 = ST.get () in
   if is_singleton h then (
     empty_list
   ) else (
@@ -430,16 +467,7 @@ let dlisthead_remove_tail #t h =
     //unlink them
     !<|= n;
     !=|> prev;
-    let y = { lhead = h.lhead ; ltail = prev ; nodes = ghost_unsnoc h.nodes } in
-    let h2 = ST.get () in
-    assert (
-      let ynodes = reveal y.nodes in
-      let hnodes = reveal h.nodes in
-      (forall (i:nat{0 <= i /\ i < Seq.length ynodes - 1 /\ i < Seq.length hnodes - 2}).
-                {:pattern (ynodes.[i]@h2)}
-         ynodes.[i]@h2 == hnodes.[i]@h1)); // OBSERVE
-    admit ();
-      y
+    { lhead = h.lhead ; ltail = prev ; nodes = ghost_unsnoc h.nodes }
   )
 
 #reset-options
@@ -449,34 +477,35 @@ let rec get_ref_index (#t:Type) (s:seq (gpointer t)) (x:gpointer t{s `contains_b
     (decreases (Seq.length s)) =
   contains_elim s x;
   let h, t = Seq.head s, Seq.tail s in
-  if compare_addrs h x then 0 else (
+  if ptr_eq h x then 0 else (
     contains_cons h t x;
     1 + get_ref_index t x)
 
-val lemma_get_ref_index : #t:Type -> s:seq (gpointer t) -> x:gpointer t{s `contains_by_addr` x} ->
-  Lemma (ensures (
-    compare_addrs s.[get_ref_index s x] x))
-    (decreases (Seq.length s))
-    [SMTPat (s.[get_ref_index s x])]
-let rec lemma_get_ref_index #t s x =
-  contains_elim s x;
-  let h, t = Seq.head s, Seq.tail s in
-  if compare_addrs h x then () else (
-    contains_cons h t x;
-    lemma_get_ref_index t x)
+// val lemma_get_ref_index : #t:Type -> s:seq (gpointer t) -> x:gpointer t{s `contains_by_addr` x} ->
+//   Lemma (ensures (
+//     g_ptr_eq s.[get_ref_index s x] x))
+//     (decreases (Seq.length s))
+//     [SMTPat (g_ptr_eq s.[get_ref_index s x] x)]
+// let rec lemma_get_ref_index #t s x =
+//   contains_elim s x;
+//   let h, t = Seq.head s, Seq.tail s in
+//   if ptr_eq h x then () else (
+//     contains_cons h t x;
+//     lemma_get_ref_index t x)
 
-val split_seq_at_element : #t:Type -> s:seq (gpointer t) -> x:gpointer t{s `contains_by_addr` x} ->
-  GTot (v:(seq (gpointer t) * nat * seq (gpointer t)){
-      let l, i, r = v in
-      indexable s i /\ (
-      s == append l (cons s.[i] r) /\
-      compare_addrs s.[i] x)
-  })
-let split_seq_at_element #t s x =
-  let i = get_ref_index s x in
-  let l, mr = Seq.split s i in
-  lemma_split s i;
-  l, i, tail mr
+// val split_seq_at_element : #t:Type -> s:seq (gpointer t) -> x:gpointer t{s `contains_by_addr` x} ->
+//   GTot (v:(seq (gpointer t) * nat * seq (gpointer t)){
+//       let l, i, r = v in
+//       indexable s i /\ (
+//       let (i:nat{i < length s}) = i in // workaround for two phase thing
+//       s == append l (cons s.[i] r) /\
+//       g_ptr_eq s.[i] x)
+//   })
+// let split_seq_at_element #t s x =
+//   let i = get_ref_index s x in
+//   let l, mr = Seq.split s i in
+//   lemma_split s i;
+//   l, i, tail mr
 
 #reset-options "--z3rlimit 1 --detail_errors --z3rlimit_factor 20"
 
@@ -495,11 +524,12 @@ let dlisthead_remove_strictly_mid #t h e =
   let h1 = ST.get () in
   let prev = (!e).blink in
   let next = (!e).flink in
+  lemma_all_elements_distinct (ST.get ()) h; // required to be able to say [prev]
+                                             //     and [next] are not same
   recall prev;
   recall next;
   !<|= e;
   !=|> e;
-  admit ();
   prev =|> next;
   prev <|= next;
   let nodes = h.nodes in // TODO: Fix this
